sdk/test/test_alethe_farkas.ml
@@ -143,6 +143,7 @@ let test_extract_g4 () =
        let kind = match other with
          | Verified -> "Verified"
          | Unknown_hypothesis _ -> "Unknown_hypothesis"
+            | Duplicate_hypothesis _ -> "Duplicate_hypothesis"
          | Nonlinear _ -> "Nonlinear"
          | Bad_coefficient _ -> "Bad_coefficient"
          | Negative_coefficient _ -> "Negative_coefficient"
@@ -168,6 +169,7 @@ let test_extract_g5 () =
        let kind = match other with
          | Verified -> "Verified"
          | Unknown_hypothesis _ -> "Unknown_hypothesis"
+            | Duplicate_hypothesis _ -> "Duplicate_hypothesis"
          | Nonlinear _ -> "Nonlinear"
          | Bad_coefficient _ -> "Bad_coefficient"
          | Negative_coefficient _ -> "Negative_coefficient"
